day 11 and some of 8

problems/11/Problem11.dfy
@@ -1,9 +1,98 @@
+include "../../parser/split.dfy"
+include "../../parser/parseInt.dfy"
+include "../../libraries/src/dafny/Collections/Seqs.dfy"
+include "../../libraries/src/Wrappers.dfy"
 module Problem11 {
+    import opened Split
+    import opened ParseInt
+    import opened Dafny.Collections.Seq
+    import opened Wrappers
+
+    type Point = (nat, nat)
+    function abs(x: int): nat {
+        if x < 0 then -x else x
+    }
+
+    predicate allEmpty(row: seq<string>) {
+        forall i :: 0 <= i < |row| ==> row[i] == "."
+    }
+
+    predicate allEmptyColumn(grid: seq<seq<string>>, x: int) {
+        forall i :: 0 <= i < |grid| ==> 0 <= x < |grid[i]| && grid[i][x] == "."
+    }
+
+    method parseInput2(input: string) returns (galaxies: seq<Point>)
+
+    {
+        var lines := splitOnBreak(input);
+        var grid := Map(x => split(x,""), Filter(x=>x != "", lines));
+        assume {:axiom} |grid| > 0;
+        var emptyrows := set i | 0 <= i < |grid| && allEmpty(grid[i]);
+        var emptycolumns := set i | 0 <= i < |grid[0]| && allEmptyColumn(grid, i);
+        var expansion := 1000000-1; //-1 to not overcount the row
+        galaxies := [];
+        for y := 0 to |grid| {
+            for x := 0 to |grid[y]| {
+                if grid[y][x] == "#" {
+                    var yoffset := |set i | 0 <= i < y && i in emptyrows | * expansion;
+                    var xoffset := |set i |  0 <= i < x && i in emptycolumns| * expansion;
+                    galaxies := galaxies + [(x+xoffset, y+yoffset)];
+                }
+            }
+        }
+    }
+
+    method parseInput(input: string) returns (galaxies: seq<Point>)
+
+    {
+        var lines := splitOnBreak(input);
+        var grid := Map(x => split(x,""), Filter(x=>x != "", lines));
+        assume {:axiom} |grid| > 0;
+        var emptyrows := set i | 0 <= i < |grid| && allEmpty(grid[i]);
+        var emptycolumns := set i | 0 <= i < |grid[0]| && allEmptyColumn(grid, i);
+        // print grid, "\n";
+        // print emptyrows, "\n";
+        // print emptycolumns, "\n";
+        galaxies := [];
+        for y := 0 to |grid| {
+            for x := 0 to |grid[y]| {
+                if grid[y][x] == "#" {
+                    var yoffset := |set i | 0 <= i < y && i in emptyrows |;
+                    var xoffset := |set i |  0 <= i < x && i in emptycolumns|;
+                    // print xoffset, " ", yoffset, "\n";
+                    // print "pt: ", (x+xoffset, y+yoffset), "\n";
+                    galaxies := galaxies + [(x+xoffset, y+yoffset)];
+                }
+            }
+        }
+    }
+
+    function distance(a: Point, b: Point): nat {
+        abs(a.0-b.0)+abs(a.1-b.1)
+    }
+
     method problem11_1(input: string) returns (x: int) {
-        return 3;
+        var galaxies := parseInput(input);
+        assume {:axiom} |galaxies| > 0;
+        // print "dist 1,7 ", distance(galaxies[0],galaxies[6]), "\n";
+        // print "dist 3,6 ", distance(galaxies[2],galaxies[5]), "\n";
+        // print "dist 8,9 ", distance(galaxies[7],galaxies[8]), "\n";
+        x := 0;
+        for i := 0 to |galaxies|-1 {
+            for j := i + 1 to |galaxies| {
+                x := x + distance(galaxies[i], galaxies[j]);
+            }
+        }
     }
 
     method problem11_2(input: string) returns (x: int) {
-        return 4;
+        var galaxies := parseInput2(input);
+        assume {:axiom} |galaxies| > 0;
+        x := 0;
+        for i := 0 to |galaxies|-1 {
+            for j := i + 1 to |galaxies| {
+                x := x + distance(galaxies[i], galaxies[j]);
+            }
+        }
     }
 }
