problems/8/Problem8.dfy
@@ -1,9 +1,113 @@
+include "../../parser/split.dfy"
+include "../../parser/parseInt.dfy"
+include "../../libraries/src/dafny/Collections/Seqs.dfy"
+include "../../libraries/src/Wrappers.dfy"
 module Problem8 {
-    method problem8_1(input: string) returns (x: int) {
-        return 3;
+    import opened Split
+    import opened ParseInt
+    import opened Dafny.Collections.Seq
+    import opened Wrappers
+    datatype Direction = Left | Right
+    datatype State = State(name: string, exits: (string, string))
+    method parseInput(input: string) returns (steps: seq<Direction>, states: seq<State>) {
+        states := [];
+        var lines := splitOnDoubleBreak(input);
+        assume {:axiom} |lines| == 2;
+        expect |lines| == 2;
+        steps := Map((letter: string) => match letter {
+            case "L" => Left
+            case "R" => Right
+            case _ => Left
+        }, split(lines[0], ""));
+        var stateLines := splitOnBreak(lines[1]);
+        for i := 0 to |stateLines| {
+            if stateLines[i] != "" {
+                assume {:axiom} |stateLines[i]| == 16;
+                expect |stateLines[i]| == 16;
+                var name := stateLines[i][0..3];
+                var le := stateLines[i][7..10];
+                var re := stateLines[i][12..15];
+                states := states + [State(name, (le, re))];
+            }
+        }
+
     }
 
-    method problem8_2(input: string) returns (x: int) {
-        return 4;
+    method problem8_1(input: string) returns (x: int) 
+        decreases *
+    {
+        var steps, states := parseInput(input);
+        assume {:axiom} |steps| > 0;
+        expect |steps| > 0;
+        var stateMap: map<string, State> := map[];
+        print steps, "\n";
+        print states, "\n";
+        for i := 0 to |states| {
+            stateMap := stateMap[states[i].name := states[i]];
+        }
+        assume {:axiom} "AAA" in stateMap;
+        expect "AAA" in stateMap;
+        var state := stateMap["AAA"];
+        var step := 0; 
+        while state.name != "ZZZ" 
+            decreases *
+        {
+            var next := match steps[step % |steps|] {
+                case Left => state.exits.0
+                case Right => state.exits.1
+            };
+
+            assume {:axiom} next in stateMap;
+            expect next in stateMap;
+            state := stateMap[next];
+            step := step + 1;
+        }
+        return step;
+    }
+
+    predicate EndState(states: seq<State>) 
+        requires forall i :: 0 <= i < |states| ==> |states[i].name| > 0;
+    {
+        forall i :: 0 <= i < |states| ==> states[i].name[|states[i].name|-1] == 'Z'
+    }
+
+    method problem8_2(input: string) returns (x: int) 
+        decreases *
+    {
+        var steps, states := parseInput(input);
+        assume {:axiom} |steps| > 0;
+        assume {:axiom} forall i :: 0 <= i < |states| ==> |states[i].name| > 0;
+        expect |steps| > 0;
+        var stateMap: map<string, State> := map[];
+        print |steps|, "\n";
+        print |states|, "\n";
+        for i := 0 to |states| {
+            stateMap := stateMap[states[i].name := states[i]];
+        }
+        var statelist: seq<State> := Filter((s: State) requires |s.name| > 0 => s.name[|s.name|-1]=='A', states);
+        var cycles: seq<set<State>> := seq(|statelist|, i => {});
+        print statelist;
+        print "Starting state Count:= ", |statelist|, "\n";
+
+        var step := 0; 
+        // while !EndState(statelist)
+        //     decreases *
+        // {
+        //     var nextList: seq<State> := [];
+        //     for i := 0 to |statelist| {
+
+        //         var next := match steps[step % |steps|] {
+        //             case Left => statelist[i].exits.0
+        //             case Right => statelist[i].exits.1
+        //         };
+
+        //         assume {:axiom} next in stateMap;
+        //         expect next in stateMap;
+        //         nextList := nextList+[stateMap[next]];
+        //     }
+        //     statelist := nextList;
+        //     step := step + 1;
+        // }
+        return step;
     }
 }
